TheoryInTerm.v
@@ -41,9 +41,9 @@ apply H; apply H0.
 Qed.
 
 Definition NatRec (f g n:term) : term.
-left; exists (fun i => NATREC (int f i) 
+left; exists (fun i => natrec (int f i) 
   (fun m t => app (app (int g i) m) t) (int n i)).
-repeat red; intros. apply NATREC_morph. 
+repeat red; intros. apply natrec_morph. 
  rewrite H; reflexivity.
  
  repeat red; intros. rewrite H, H0, H1. reflexivity.
@@ -71,15 +71,15 @@ set (fS := int g i) in *; clearbody fS.
 
 elim H using N_ind; intros. 
  revert H6. apply in_set_morph.
-  apply NATREC_morph.
+  apply natrec_morph.
    reflexivity.
    do 2 red; intros. rewrite H7. rewrite H6. reflexivity.
    symmetry; assumption.
   rewrite H5; reflexivity.
 
- rewrite NATREC_0. apply H1.
+ rewrite natrec_0. apply H1.
  
- rewrite NATREC_Succ; auto.
+ rewrite natrec_S; auto.
   refine (let H6 := prod_elim _ _ _ _ _ H2 H4 in _).
    red; intros. apply prod_ext.
     apply app_ext; try assumption.
@@ -106,9 +106,9 @@ elim H using N_ind; intros.
   simpl in H7. revert H7. apply in_set_morph; try reflexivity.
   set (fS' := fun n y => app (app fS n) y) in |-*.
    apply app_ext; try reflexivity.
-    replace (fun k : nat => V.cons (NATREC f0 fS' n0) 
+    replace (fun k : nat => V.cons (natrec f0 fS' n0) 
                                        (V.cons n0 i) k) 
-    with (V.cons (NATREC f0 fS' n0) (V.cons n0 i)); trivial.
+    with (V.cons (natrec f0 fS' n0) (V.cons n0 i)); trivial.
     rewrite simpl_int_lift. symmetry; apply simpl_int_lift1.
 
   do 3 red; intros. rewrite H6, H7; reflexivity.
@@ -116,9 +116,9 @@ Qed.
 
 Definition Add : term -> term -> term.
 intros m n; left; 
-exists (fun i => NATREC (int m i) (fun _ => succ) (int n i)).
+exists (fun i => natrec (int m i) (fun _ => succ) (int n i)).
 do 2 red; intros. 
-apply NATREC_morph; try rewrite H; try reflexivity.
+apply natrec_morph; try rewrite H; try reflexivity.
  do 2 red; intros. rewrite H1; reflexivity.
 Defined.
 
@@ -130,21 +130,21 @@ do 2 red in H0; simpl in H0; specialize H0 with (1:=H1).
 do 2 red in H; simpl in H; specialize H with (1:=H1).
 elim H0 using N_ind; intros.
  revert H4; apply in_set_morph; try reflexivity.
-  apply NATREC_morph; try reflexivity; try symmetry; trivial.
+  apply natrec_morph; try reflexivity; try symmetry; trivial.
    do 2 red; intros; rewrite H5; reflexivity.
    
- rewrite NATREC_0; trivial.
+ rewrite natrec_0; trivial.
 
- rewrite NATREC_Succ; trivial.
+ rewrite natrec_S; trivial.
   apply succ_typ; trivial.
     
   do 3 red; intros. rewrite H5; reflexivity.
 Qed.
 
 Definition ind_schema_term : term.
-left; exists (fun i => NATREC (i 2) (fun n x => app (app (i 1) n) x) (i 0)).
+left; exists (fun i => natrec (i 2) (fun n x => app (app (i 1) n) x) (i 0)).
 do 2 red; intros.
-apply NATREC_morph; try apply H.
+apply natrec_morph; try apply H.
  do 2 red; intros; simpl. apply app_ext; trivial.
   apply app_ext; trivial.
 Defined.
@@ -155,7 +155,7 @@ Lemma discr_term : forall e n i, val_ok e i ->
   ~ eq_typ e Zero (Add n (Succ Zero)).
 red; intros. red in H0; simpl in *.
 specialize H0 with (1 := H).
- rewrite NATREC_Succ in H0. rewrite NATREC_0 in H0.
+ rewrite natrec_S in H0. rewrite natrec_0 in H0.
  symmetry in H0; apply discr in H0. trivial.
 
  do 3 red; intros. rewrite H2; reflexivity.
@@ -172,13 +172,13 @@ specialize H0 with (1:=H2).
 specialize H1 with (1:=H2).
 assert (morph2 (fun _ => succ)).
  do 3 red; intros x0 y0 H3 x1 y1 H4; rewrite H4; reflexivity.
-do 2 rewrite NATREC_Succ in H1; try apply zero_typ; try apply H3.
-do 2 rewrite NATREC_0 in H1.
+do 2 rewrite natrec_S in H1; try apply zero_typ; try apply H3.
+do 2 rewrite natrec_0 in H1.
 apply succ_inj; trivial.
 Qed.
  
 Lemma Add_0 : forall e n, typ e n T -> eq_typ e (Add n Zero) n.
-destruct n; red; intros; simpl; rewrite NATREC_0; reflexivity.
+destruct n; red; intros; simpl; rewrite natrec_0; reflexivity.
 Qed.
 
 Lemma Add_ass : forall e x y, typ e y T ->
@@ -187,10 +187,10 @@ assert (morph2 (fun _ => succ)).
  do 3 red; intros x y H0 x1 y1 H1; rewrite H1; reflexivity.
 do 2 red; intros; simpl.
 replace (fun k : nat => i k) with i; trivial.
-do 2 rewrite (NATREC_Succ _ _ _ H zero_typ).
+do 2 rewrite (natrec_S _ _ _ H zero_typ).
 red in H0; simpl in H0; specialize H0 with (1:=H1).
-do 2 rewrite NATREC_0. 
-rewrite (NATREC_Succ _ _ _ H H0); reflexivity.
+do 2 rewrite natrec_0. 
+rewrite (natrec_S _ _ _ H H0); reflexivity.
 Qed.
 
 
@@ -604,7 +604,7 @@ apply Fall_intro.
   assert (nth_error (EQ_trm Zero (Add (Ref 0) (Succ Zero))::T::e) 
     0 = value (EQ_trm Zero (Add (Ref 0) (Succ Zero)))); trivial.
   specialize H with (1:=H0). clear H0. red in H; simpl in H.
-  rewrite NATREC_Succ in H.
+  rewrite natrec_S in H.
    rewrite EQ_discr in H. apply empty_ax in H; contradiction.
 
    do 2 red; intros _ _ _ x1 x2 H1; rewrite H1; reflexivity.
@@ -659,8 +659,8 @@ apply Fall_intro.
      rewrite H in H0P; simpl in H0P. rewrite H0; simpl.
      assert (morph2 (fun _ : set => succ)).
       do 3 red; intros. rewrite H8; reflexivity.
-     do 2 rewrite (NATREC_Succ _ _ _ H7 zero_typ) in H0P.
-     do 2 rewrite NATREC_0 in H0P. simpl in H0P.
+     do 2 rewrite (natrec_S _ _ _ H7 zero_typ) in H0P.
+     do 2 rewrite natrec_0 in H0P. simpl in H0P.
      apply EQ_succ_inj with (x0 := i 0); trivial.
     
      rewrite H in H6; simpl in H6; discriminate.
@@ -811,12 +811,12 @@ apply Impl_intro.
       rewrite int_lift_rec_eq. rewrite <- V.cons_lams; simpl.
        2 : do 2 red; intros x y H3; rewrite H3; reflexivity.
 
-       rewrite NATREC_Succ. 
+       rewrite natrec_S. 
         2 : do 3 red; intros _ _ _ m0 n0 Hmn; rewrite Hmn; reflexivity.
 
         2: apply zero_typ.
 
-       rewrite NATREC_0. rewrite <- H0. rewrite <- V.cons_lams.
+       rewrite natrec_0. rewrite <- H0. rewrite <- V.cons_lams.
         2 : do 2 red; intros m0 n0 Hmn; rewrite Hmn; reflexivity.
 
         apply int_morph; try reflexivity.
@@ -841,7 +841,7 @@ apply Impl_intro.
      rewrite V.lams0. 
      replace (fun k : nat => V.shift 1 i k) with (V.shift 1 i); trivial.
      rewrite (Hsplit i). elim Hind using N_ind.
-      intros. rewrite NATREC_morph.
+      intros. rewrite natrec_morph.
        rewrite <- H0. apply H1.
      
        reflexivity.
@@ -851,9 +851,9 @@ apply Impl_intro.
 
        symmetry; trivial.
 
-     rewrite NATREC_0; trivial.
+     rewrite natrec_0; trivial.
 
-     intros. rewrite NATREC_Succ; trivial.
+     intros. rewrite natrec_S; trivial.
       generalize prod_elim; intro Haux.
       specialize Haux with (2:=Hsucc) (3:=H). simpl in Haux.
       assert (eq_fun N
